src/HOL/Hoare/ExamplesAbort.thy
@@ -4,26 +4,27 @@
     Copyright   1998 TUM
 
 Some small examples for programs that may abort.
-Currently only show the absence of abort.
 *)
 
 theory ExamplesAbort = HoareAbort:
 
-syntax guarded_com :: "'bool \<Rightarrow> 'a com \<Rightarrow> 'a com"  ("_ \<rightarrow> _" 60)
-translations "P \<rightarrow> c" == "IF P THEN c ELSE Abort FI"
-
 lemma "VARS x y z::nat
  {y = z & z \<noteq> 0} z \<noteq> 0 \<rightarrow> x := y div z {x = 1}"
 by vcg_simp
+
+lemma
+ "VARS a i j
+ {k <= length a & i < k & j < k} j < length a \<rightarrow> a[i] := a!j {True}"
+apply vcg_simp
+apply arith
+done
 
 lemma "VARS (a::int list) i
  {True}
  i := 0;
  WHILE i < length a
  INV {i <= length a}
- DO i < length a \<rightarrow> a := a[i := 7];
-    i := i+1
- OD
+ DO a[i] := 7; i := i+1 OD
  {True}"
 apply vcg_simp
 apply arith
