src/HOL/Hoare/HeapSyntaxAbort.thy
@@ -1,0 +1,47 @@
+(*  Title:      HOL/Hoare/HeapSyntax.thy
+    ID:         $Id$
+    Author:     Tobias Nipkow
+    Copyright   2002 TUM
+*)
+
+theory HeapSyntaxAbort = HoareAbort + Heap:
+
+subsection "Field access and update"
+
+text{* Heap update @{text"p^.h := e"} is now guarded against @{term p}
+being Null. However, @{term p} may still be illegal,
+e.g. uninitialized or dangling. To guard against that, one needs a
+more detailed model of the heap where allocated and free addresses are
+distinguished, e.g. by making the heap a map, or by carrying the set
+of free addresses around. This is needed anyway as soon as we want to
+reason about storage allocation/deallocation. *}
+
+syntax
+  "refupdate" :: "('a \<Rightarrow> 'b) \<Rightarrow> 'a ref \<Rightarrow> 'b \<Rightarrow> ('a \<Rightarrow> 'b)"
+   ("_/'((_ \<rightarrow> _)')" [1000,0] 900)
+  "@fassign"  :: "'a ref => id => 'v => 's com"
+   ("(2_^._ :=/ _)" [70,1000,65] 61)
+  "@faccess"  :: "'a ref => ('a ref \<Rightarrow> 'v) => 'v"
+   ("_^._" [65,1000] 65)
+translations
+  "refupdate f r v"  ==  "f(addr r := v)"
+  "p^.f := e"  =>  "(p \<noteq> Null) \<rightarrow> (f := refupdate f p e)"
+  "p^.f"       =>  "f(addr p)"
+
+
+declare fun_upd_apply[simp del] fun_upd_same[simp] fun_upd_other[simp]
+
+
+text "An example due to Suzuki:"
+
+lemma "VARS v n
+  {w = Ref w0 & x = Ref x0 & y = Ref y0 & z = Ref z0 &
+   distinct[w0,x0,y0,z0]}
+  w^.v := (1::int); w^.n := x;
+  x^.v := 2; x^.n := y;
+  y^.v := 3; y^.n := z;
+  z^.v := 4; x^.n := z
+  {w^.n^.n^.v = 4}"
+by vcg_simp
+
+end
