src/HOL/Hoare/Pointer_ExamplesAbort.thy
@@ -1,0 +1,30 @@
+(*  Title:      HOL/Hoare/Pointer_ExamplesAbort.thy
+    ID:         $Id$
+    Author:     Tobias Nipkow
+    Copyright   2002 TUM
+
+Examples of verifications of pointer programs
+*)
+
+theory Pointer_ExamplesAbort = HeapSyntaxAbort:
+
+section "Verifications"
+
+subsection "List reversal"
+
+text "Interestingly, this proof is the same as for the unguarded program:"
+
+lemma "VARS tl p q r
+  {List tl p Ps \<and> List tl q Qs \<and> set Ps \<inter> set Qs = {}}
+  WHILE p \<noteq> Null
+  INV {\<exists>ps qs. List tl p ps \<and> List tl q qs \<and> set ps \<inter> set qs = {} \<and>
+                 rev ps @ qs = rev Ps @ Qs}
+  DO r := p; (p \<noteq> Null \<rightarrow> p := p^.tl); r^.tl := q; q := r OD
+  {List tl q (rev Ps @ Qs)}"
+apply vcg_simp
+  apply fastsimp
+ apply(fastsimp intro:notin_List_update[THEN iffD2])
+apply fastsimp
+done
+
+end
