src/HOL/Hoare/Separation.thy
@@ -6,21 +6,27 @@ types heap = "(nat \<Rightarrow> nat option)"
 text{* The semantic definition of a few connectives: *}
 
 constdefs
- R:: "heap \<Rightarrow> heap \<Rightarrow> heap \<Rightarrow> bool"
-"R h h1 h2 == dom h1 \<inter> dom h2 = {} \<and> h = h1 ++ h2"
+ ortho:: "heap \<Rightarrow> heap \<Rightarrow> bool" (infix "\<bottom>" 55)
+"h1 \<bottom> h2 == dom h1 \<inter> dom h2 = {}"
 
- star:: "(heap \<Rightarrow> bool) \<Rightarrow> (heap \<Rightarrow> bool) \<Rightarrow> (heap \<Rightarrow> bool)"
-"star P Q == \<lambda>h. \<exists>h1 h2. R h h1 h2 \<and> P h1 \<and> Q h2"
+ is_empty :: "heap \<Rightarrow> bool"
+"is_empty h == h = empty"
 
  singl:: "heap \<Rightarrow> nat \<Rightarrow> nat \<Rightarrow> bool"
 "singl h x y == dom h = {x} & h x = Some y"
+
+ star:: "(heap \<Rightarrow> bool) \<Rightarrow> (heap \<Rightarrow> bool) \<Rightarrow> (heap \<Rightarrow> bool)"
+"star P Q == \<lambda>h. \<exists>h1 h2. h = h1++h2 \<and> h1 \<bottom> h2 \<and> P h1 \<and> Q h2"
+
+ wand:: "(heap \<Rightarrow> bool) \<Rightarrow> (heap \<Rightarrow> bool) \<Rightarrow> (heap \<Rightarrow> bool)"
+"wand P Q == \<lambda>h. \<forall>h'. h' \<bottom> h \<and> P h' \<longrightarrow> Q(h++h')"
 
 lemma "VARS x y z w h
  {star (%h. singl h x y) (%h. singl h z w) h}
  SKIP
  {x \<noteq> z}"
 apply vcg
-apply(auto simp:star_def R_def singl_def)
+apply(auto simp:star_def ortho_def singl_def)
 done
 
 text{* To suppress the heap parameter of the connectives, we assume it
@@ -32,45 +38,110 @@ may bind the implicit H. *}
 text{* Nice input syntax: *}
 
 syntax
+ "@emp" :: "bool" ("emp")
  "@singl" :: "nat \<Rightarrow> nat \<Rightarrow> bool" ("[_ \<mapsto> _]")
  "@star" :: "bool \<Rightarrow> bool \<Rightarrow> bool" (infixl "**" 60)
+ "@wand" :: "bool \<Rightarrow> bool \<Rightarrow> bool" (infixl "-o" 60)
 
 ML{*
+(* free_tr takes care of free vars in the scope of sep. logic connectives:
+   they are implicitly applied to the heap *)
+fun free_tr(t as Free _) = t $ Syntax.free "H"
+  | free_tr t = t
+
+fun emp_tr [] = Syntax.const "is_empty" $ Syntax.free "H"
+  | emp_tr ts = raise TERM ("emp_tr", ts);
 fun singl_tr [p,q] = Syntax.const "singl" $ Syntax.free "H" $ p $ q
   | singl_tr ts = raise TERM ("singl_tr", ts);
 fun star_tr [P,Q] = Syntax.const "star" $
-      absfree("H",dummyT,P) $ absfree("H",dummyT,Q) $ Syntax.free "H"
+      absfree("H",dummyT,free_tr P) $ absfree("H",dummyT,free_tr Q) $
+      Syntax.free "H"
   | star_tr ts = raise TERM ("star_tr", ts);
+fun wand_tr [P,Q] = Syntax.const "wand" $
+      absfree("H",dummyT,P) $ absfree("H",dummyT,Q) $ Syntax.free "H"
+  | wand_tr ts = raise TERM ("wand_tr", ts);
 *}
 
-parse_translation {* [("@singl", singl_tr),("@star", star_tr)] *}
+parse_translation
+ {* [("@emp", emp_tr), ("@singl", singl_tr),
+     ("@star", star_tr), ("@wand", wand_tr)] *}
 
 lemma "VARS H x y z w
  {[x\<mapsto>y] ** [z\<mapsto>w]}
  SKIP
  {x \<noteq> z}"
 apply vcg
-apply(auto simp:star_def R_def singl_def)
+apply(auto simp:star_def ortho_def singl_def)
+done
+
+lemma "VARS H x y z w
+ {emp ** emp}
+ SKIP
+ {emp}"
+apply vcg
+apply(auto simp:star_def ortho_def is_empty_def)
 done
 
 text{* Nice output syntax: *}
 
 ML{*
+local
+fun strip (Abs(_,_,(t as Free _) $ Bound 0)) = t
+  | strip (Abs(_,_,(t as Var _) $ Bound 0)) = t
+  | strip (Abs(_,_,P)) = P
+  | strip (Const("is_empty",_)) = Syntax.const "@emp"
+  | strip t = t;
+in
+fun is_empty_tr' [_] = Syntax.const "@emp"
 fun singl_tr' [_,p,q] = Syntax.const "@singl" $ p $ q
-fun star_tr' [Abs(_,_,P),Abs(_,_,Q),_] = Syntax.const "@star" $ P $ Q
+fun star_tr' [P,Q,_] = Syntax.const "@star" $ strip P $ strip Q
+fun wand_tr' [P,Q,_] = Syntax.const "@wand" $ strip P $ strip Q
+end
 *}
 
-print_translation {* [("singl", singl_tr'),("star", star_tr')] *}
+print_translation
+ {* [("is_empty", is_empty_tr'),("singl", singl_tr'),("star", star_tr')] *}
 
 lemma "VARS H x y z w
  {[x\<mapsto>y] ** [z\<mapsto>w]}
  y := w
  {x \<noteq> z}"
 apply vcg
-apply(auto simp:star_def R_def singl_def)
+apply(auto simp:star_def ortho_def singl_def)
 done
 
+lemma "VARS H x y z w
+ {emp ** emp}
+ SKIP
+ {emp}"
+apply vcg
+apply(auto simp:star_def ortho_def is_empty_def)
+done
 
+(* move to Map.thy *)
+lemma override_comm: "dom m1 \<inter> dom m2 = {} \<Longrightarrow> m1++m2 = m2++m1"
+apply(rule ext)
+apply(fastsimp simp:override_def split:option.split)
+done
+
+(* a law of separation logic *)
+(* something is wrong with the pretty printer, but I cannot figure out what. *)
+
+lemma star_comm: "P ** Q = Q ** P"
+apply(simp add:star_def ortho_def)
+apply(blast intro:override_comm)
+done
+
+lemma "VARS H x y z w
+ {P ** Q}
+ SKIP
+ {Q ** P}"
+apply vcg
+apply(simp add: star_comm)
+done
+
+end
+(*
 consts llist :: "(heap * nat)set"
 inductive llist
 intros
@@ -86,5 +157,4 @@ apply(rule_tac "h1.0" = "%n. if n=q then Some p else None" in llist.cons)
 prefer 3 apply assumption
 prefer 2 apply(simp add:singl_def dom_def)
 apply(simp add:R_def dom_def)
-
-
+*)
